

Simplification

$$\textcircled{a} \quad AB + A(B+C) + B(B+C)$$

$$= (AB + AB) + AC + B + BC$$

$$= AB + AC + B(1+C)$$

$$= AB + AC + B \cdot 1$$

$$= B + AB + AC$$

$$= B(1+A) + AC$$

$$= B + AC$$

$$\textcircled{b} \quad A'B + BC' + BC + AB'C'$$

$$= A'B + B(C+C') + AB'C'$$

$$= A'B + B + AB'C'$$

$$= B(A+1) + AB'C'$$

$$= B + AB'C'$$

$$= B'(A+B+C)$$

$$= A'B' + B'B + B'C$$

$$= A'B' + B'C$$

$$= B'(A+C)$$

$$= B + AC'$$

$$\textcircled{c} \quad (X + Y' + Z')(X + Y' + Z)(X + Y + Z')$$

$$= (X + \underline{XY'} + XZ + \underline{XY'} + Y' + ZY' + XZ' + Y'Z')(X + Y + Z')$$

$$= (X + \underline{XY'} + \underline{XZ} + Y' + ZY' + \underline{XZ'} + Y'Z')(X + Y + Z')$$

$$= (X(1+Y') + X(Z+Z') + Y'(1+Z) + Y'Z')(X + Y + Z')$$

$$= (x + x + y' + y'z')(x + y + z')$$

$$= (x + y'(1 + z'))(x + y + z')$$

$$= (x + y')(x + y + z')$$

$$= x + xy + \underline{xz'} + xy' + y'z'$$

$$= x(1 + y) + xz' + xy' + y'z'$$

$$= x(1 + z') + xy' + y'z'$$

$$= x(1 + y') + y'z'$$

$$= x + y'z'$$

$$= x + (y + z)'$$